theories/L1g/instances.v
@@ -78,9 +78,10 @@ Instance certiL1g: CerticoqLanguage (Program L1g.compile.Term):= {}.
 Local Generalizable Variable Lj.
 
 Definition translateTo `{F:utils.Fuel} `{CerticoqTranslation (Program L1g.compile.Term) Lj}
-  (p:Template.Ast.program): exception Lj :=
-  let l1g:= L1g.compile.program_Program p in
-  translate (Program L1g.compile.Term) Lj l1g.
+           (p:Template.Ast.program): exception Lj :=
+  (AstCommon.timePhase "L1 to L2")
+    (fun (_:Datatypes.unit) => (let l1g:= L1g.compile.program_Program p in
+     translate (Program L1g.compile.Term) Lj l1g)).
 
 Arguments translateTo {F} Lj {H} p.
 
