theories/common/AstCommon.v
@@ -561,6 +561,9 @@ Definition cnstrArity (p:environ) (i:inductive) (cndx:nat) :
 End trm_Sec.
 
 (* Timing facilities, instanciated by extraction in extraction.v *)
-Variable (timePhase: forall A, string -> A -> A).
 
-Axiom timePhase_id: forall {A:Type} s (x:A), timePhase s x = x.
+
+
+Variable (timePhase: forall A, string -> (Datatypes.unit -> A) -> A).
+
+Axiom timePhase_id: forall {A:Type} s (x:Datatypes.unit -> A), timePhase s x = x tt.
